src/Manifest/Manifest.v
@@ -565,6 +565,4 @@ Module ManifestTerm.
   End ClassExp.
    *)
   
-
-
 End ManifestTerm.
